CC: add constructors in Exp

Semantic/CC/Syntax/Exp.lean
@@ -10,7 +10,8 @@ inductive Exp : Sig -> Type where
 | var : Var .var s -> Exp s
 | abs : Ty .capt s -> Exp (s,x) -> Exp s
 | tabs : Ty .shape s -> Exp (s,X) -> Exp s
-| cabs : Exp (s,C) -> Exp s
+| cabs : CaptureBound s -> Exp (s,C) -> Exp s
+| pack : CaptureSet s -> Var .var s -> Exp s
 | app : Var .var s -> Var .var s -> Exp s
 | tapp : Var .var s -> Ty .shape s -> Exp s
 | capp : Var .var s -> CaptureSet s -> Exp s
@@ -21,7 +22,8 @@ def Exp.rename : Exp s1 -> Rename s1 s2 -> Exp s2
 | .var x, f => .var (x.rename f)
 | .abs T e, f => .abs (T.rename f) (e.rename (f.lift))
 | .tabs T e, f => .tabs (T.rename f) (e.rename (f.lift))
-| .cabs e, f => .cabs (e.rename (f.lift))
+| .cabs cb e, f => .cabs (cb.rename f) (e.rename (f.lift))
+| .pack cs x, f => .pack (cs.rename f) (x.rename f)
 | .app x y, f => .app (x.rename f) (y.rename f)
 | .tapp x T, f => .tapp (x.rename f) (T.rename f)
 | .capp x cs, f => .capp (x.rename f) (cs.rename f)
@@ -44,7 +46,7 @@ def Exp.rename_id {e : Exp s} : e.rename (Rename.id) = e := by
     <;> try (solve
       | rfl
       | simp [Exp.rename, Ty.rename_id, Var.rename_id,
-              CaptureSet.rename_id, Rename.lift_id]
+              CaptureSet.rename_id, CaptureBound.rename_id, Rename.lift_id]
         try aesop)
 
 theorem Var.rename_comp {x : Var k s1} {f : Rename s1 s2} {g : Rename s2 s3} :
@@ -57,7 +59,7 @@ theorem Exp.rename_comp {e : Exp s1} {f : Rename s1 s2} {g : Rename s2 s3} :
     <;> try (solve
       | rfl
       | simp [Exp.rename, Ty.rename_comp, Var.rename_comp,
-              CaptureSet.rename_comp, Rename.lift_comp]
+              CaptureSet.rename_comp, CaptureBound.rename_comp, Rename.lift_comp]
         try aesop)
 
 theorem Var.weaken_rename_comm {x : Var k s1} {f : Rename s1 s2} :
